\documentclass[10pt,a4paper]{article}

\usepackage{color}
\usepackage{psfrag,graphicx,verbatim,array,multicol,palatino,enumerate}
\usepackage{amsmath,amsfonts,bm,rotating,natbib}
\usepackage{epsfig}

\begin{document}

\begin{flushleft}
Course No. Stat 433 \\
\today
\end{flushleft}

\begin{center}
{\Large{\bf  Homework 13 Solution}}
\end{center}


\begin{flushleft}
\textbf{Page 497 Question 2.4}\\
Let $\tau_z$ be the hitting time of $z$.
\begin{eqnarray*}
P(M(t) \geq z, B(t) \leq x) &=& P(\tau_z \leq t, B(t) \leq x)\\
&=& P(\tau_z \leq x, z - (B(t) - z) \leq x) \\
&=& P(\tau_z \leq x, B(t) \geq 2z - x) \\
&=& P(B(t) \geq 2z - x) \\
&=& 1 - \Phi(\frac{2z-x}{\sqrt{t}})\\
\end{eqnarray*}
Differential with respect to $x$. \\
\begin{center}
$\frac{1}{\sqrt{2\pi t}}\exp(-\frac{1}{2}\frac{(2z-x)^2}{t}) =
\frac{1}{\sqrt{t}}\Phi(\frac{2z-x}{\sqrt{t}})$\end{center}

Then taking the derivative with respect to $z$, we get
\begin{center}
$\frac{1}{\sqrt{t}}\Phi(\frac{2z-x}{\sqrt{t}})(\frac{-2(2z-x)}{\sqrt{t}})$
\end{center}



\textbf{Page 506 Question 3.2}\\

\begin{eqnarray*}
f(B(t)=x)|B(1)=b) & = & \frac{f(B(t)=x,B(1)=b)}{f(B(1)=b)} \\
& = & \frac{f(B(t)=x)f(B(1-t)=b-x)}{f(B(1)=b)} \\
& = &
\frac{1}{\sqrt{2\pi t(1-t)}}\exp(-\frac{x^2}{2t}-\frac{(b-x)^2}{2(1-t)}+\frac{b^2}{2}) \\
& = & \frac{1}{\sqrt{2\pi t(1-t)}}\exp(-\frac{(x-tb)^2}{2t(1-t)})
\end{eqnarray*}
\begin{eqnarray*}
\\
\end{eqnarray*}

\textbf{Page 506 Question 3.8}\\

Reflected Brownian Motion has transition density
$$p(y,t|x)=\phi_{t}(y-x)+\phi_{t}(y+x) \cdots (1)$$
We know $\phi_{t}(y-x)$ satisfies the diffusion equation. In the
same way of Page 487, Exercise 1.3, we can show $\phi_{t}(y+x)$
satisfies the diffusion equation. Hence, (1) satisfies (1.3).

\begin{eqnarray*}
\\
\end{eqnarray*}



\end{flushleft}
\end{document}
